gol_rulesScript.sml
@@ -5,6 +5,8 @@ open preamble;
 
 val _ = new_theory "gol_rules";
 
+Overload "U"[local] = “BIGUNION”;
+
 (* There is an unbounded 2D plane of cells *)
 Type state[pp] = “:(int # int) set”;
 
@@ -167,7 +169,7 @@ Definition mods_wf_def:
 End
 
 Definition join_def:
-  join c1 c2  =
+  join c1 c2 =
     λn. <| area           := (c1 n).area ∪ (c2 n).area ;
            deletions      := (c1 n).deletions ∪ (c2 n).deletions ;
            insertions     := (c1 n).insertions ∪ (c2 n).insertions ;
@@ -189,6 +191,7 @@ Proof
   \\ last_x_assum drule_all
   \\ rename [‘_ (u1 ∪ u2) (_ ∪ _)’]
   \\ disch_then $ irule_at Any
+
   \\ gvs [mod_step_def,join_def]
   \\ gvs [infl_union,mods_wf_def,disjoint_mods_def,disjoint_mod_def]
   \\ rpt $ first_x_assum $ qspec_then ‘n’ assume_tac
@@ -200,6 +203,94 @@ Proof
   \\ ‘u2 ⊆ infl s2’ by gvs [step_SUBSET_infl,Abbr‘u2’]
   \\ gvs [IN_DISJOINT,EXTENSION,SUBSET_DEF]
   \\ metis_tac []
+QED
+
+Definition join_all_def:
+  join_all cst =
+    λn. <| area           := U { (c n).area           | ∃s t. (c,s,t) ∈ cst } ;
+           deletions      := U { (c n).deletions      | ∃s t. (c,s,t) ∈ cst } ;
+           insertions     := U { (c n).insertions     | ∃s t. (c,s,t) ∈ cst } ;
+           assert_area    := U { (c n).assert_area    | ∃s t. (c,s,t) ∈ cst } ;
+           assert_content := U { (c n).assert_content | ∃s t. (c,s,t) ∈ cst } |>
+End
+
+Theorem infl_bigunion:
+  infl (U ss) = U { infl s | s ∈ ss }
+Proof
+  cheat
+QED
+
+Theorem infl_compose_bigunion:
+  (∀x y. x ∈ ss ∧ y ∈ ss ∧ x ≠ y ⇒ DISJOINT (infl x) (infl y))
+  ⇒
+  step (U ss) = U { step s | s ∈ ss }
+Proof
+  cheat
+QED
+
+Theorem mod_steps_compose_bigunion:
+  ∀k cst n.
+    (∀x y. x ∈ cst ∧ y ∈ cst ∧ x ≠ y ⇒ disjoint_mods (FST x) (FST y)) ∧
+    (∀c s t. (c,s,t) ∈ cst ⇒ mods_wf c ∧ mod_steps k c n s t)
+    ⇒
+    mod_steps k (join_all cst) n
+                (U { s | ∃c t. (c,s,t) ∈ cst })
+                (U { t | ∃c s. (c,s,t) ∈ cst })
+Proof
+  Induct \\ gvs [mod_steps_def]
+  >-
+   (rw [] \\ simp [Once EXTENSION]
+    \\ rw [] \\ eq_tac \\ rw []
+    \\ res_tac \\ gvs [PULL_EXISTS]
+    \\ first_x_assum $ irule_at Any \\ gvs [])
+  \\ rpt strip_tac \\ gvs []
+  \\ qabbrev_tac ‘cst1 = { (c,s1,t) | ∃s. (c,s,t) ∈ cst ∧ mod_step (c n) s s1 }’
+  \\ last_x_assum $ qspecl_then [‘cst1’,‘n+1’] mp_tac
+  \\ impl_tac
+  >- cheat
+  \\ strip_tac
+  \\ ‘∀t. (∃c s. (c,s,t) ∈ cst1) ⇔ (∃c s. (c,s,t) ∈ cst)’ by cheat
+  \\ gvs [] \\ pop_assum kall_tac
+  \\ ‘join_all cst1 = join_all cst’ by cheat
+  \\ gvs [] \\ pop_assum kall_tac
+  \\ pop_assum $ irule_at Any
+  \\ gvs [Abbr‘cst1’]
+  \\ gvs [mod_step_def,join_all_def,infl_bigunion]
+  \\ DEP_REWRITE_TAC [infl_compose_bigunion]
+  \\ rpt conj_tac
+  >-
+   (gvs [] \\ rpt strip_tac
+    \\ first_x_assum (fn th => qspec_then ‘c’ mp_tac th \\ qspec_then ‘c'’ mp_tac th)
+    \\ disch_then $ drule_then strip_assume_tac
+    \\ disch_then $ drule_then strip_assume_tac
+    \\ last_x_assum $ dxrule_then $ dxrule
+    \\ gvs [disjoint_mods_def]
+    \\ gvs [disjoint_mod_def]
+    \\ disch_then $ qspec_then ‘n’ assume_tac
+    \\ metis_tac [IN_DISJOINT,SUBSET_DEF])
+  >-
+   (gvs [SUBSET_DEF] \\ rw []
+    \\ first_x_assum $ drule_then $ strip_assume_tac
+    \\ gvs [PULL_EXISTS]
+    \\ last_x_assum $ irule_at $ Pos last \\ gvs [])
+  >-
+   (gvs [mods_wf_def,mod_wf_def]
+    \\ irule EQ_TRANS
+    \\ qexists_tac ‘U {step s ∩ (c n).assert_area | (∃c t. (c,s,t) ∈ cst)}’
+    \\ conj_tac
+    >- cheat
+    \\ cheat)
+  \\ cheat
+QED
+
+Theorem run_compose_bigunion:
+  ∀k cst n.
+    (∀x y. x ∈ cst ∧ y ∈ cst ∧ x ≠ y ⇒ disjoint_mods (FST x) (FST y)) ∧
+    (∀c s t. (c,s,t) ∈ cst ⇒ mods_wf c ∧ run c s)
+    ⇒
+    run (join_all cst) (U { s | ∃c t. (c,s,t) ∈ cst })
+Proof
+  cheat (* true if the above is *)
 QED
 
 (*
@@ -243,6 +334,286 @@ Proof
   \\ IF_CASES_TAC \\ gvs []
   \\ gvs [EXTENSION,SUBSET_DEF]
   \\ metis_tac []
+QED
+
+Theorem to_assert_run:
+  ∀c s.
+    run c s ∧
+    can_assert p c
+    ⇒
+    run (assert p c) s
+Proof
+  rw [run_def,run_to_def]
+  \\ last_x_assum $ qspec_then ‘k’ strip_assume_tac
+  \\ drule_all to_assert
+  \\ disch_then $ irule_at Any
+QED
+
+(*
+  deletions and insertions --> nop
+*)
+
+Definition del_io_mod_def:
+  del_io_mod p m =
+    if p ∩ m.deletions = EMPTY then m else
+      m with <| assert_area := m.assert_area DIFF p ;
+                assert_content := m.assert_content DIFF p ;
+                insertions := m.insertions DIFF p ;
+                deletions := m.deletions DIFF p |>
+End
+
+Definition del_io_def:
+  del_io p c = λn. del_io_mod p (c n)
+End
+
+Theorem to_del_io:
+  ∀k n s t.
+    mod_steps k c n s t ∧
+    can_assert p c
+    ⇒
+    mod_steps k (del_io p c) n s t
+Proof
+  Induct
+  \\ gvs [mod_steps_def,PULL_EXISTS]
+  \\ rpt strip_tac \\ gvs []
+  \\ last_x_assum $ drule_then $ irule_at Any
+  \\ gvs [can_assert_def]
+  \\ first_x_assum $ qspec_then ‘n’ assume_tac
+  \\ gvs [mod_step_def,del_io_def,del_io_mod_def]
+  \\ IF_CASES_TAC \\ gvs []
+  \\ gvs [EXTENSION,SUBSET_DEF]
+  \\ metis_tac []
+QED
+
+Theorem to_assert_run:
+  ∀c s.
+    run c s ∧
+    can_assert p c
+    ⇒
+    run (del_io p c) s
+Proof
+  rw [run_def,run_to_def]
+  \\ last_x_assum $ qspec_then ‘k’ strip_assume_tac
+  \\ drule_all to_del_io
+  \\ disch_then $ irule_at Any
+QED
+
+(*
+  translate by dx dy
+*)
+
+(*
+  circuit conventions (set and list versions)
+   - uses 75x75 coordinates
+*)
+
+Definition box_def:
+  box (x:int,y:int) (w:num,h:num) = { (x + &i, y + &j) | i < w ∧ j < h }
+End
+
+Definition base_area_def:
+  base_area area =
+    U { box (75 * x - 75, 75 * y - 75) (150,150) | (x,y) ∈ area }
+End
+
+Definition io_box_def:
+  io_box (x:int, y:int) =
+    box (75 * x - 6, 75 * y - 6) (12, 12)
+End
+
+Datatype:
+  dir = N | S | W | E
+End
+
+Definition circ_mod_wf_def:
+  circ_mod_wf area ins outs as ⇔
+    (∀x y. (x,y) ∈ area ⇒ x % 2 = 0 ∧ y % 2 = 0) ∧
+    (∀x y r. ((x,y),r) ∈ ins ∪ outs ∪ as ⇒ ((x % 2 = 0) ≠ (y % 2 = 0))) ∧
+    (∀x y r1 r2. ((x,y),r1) ∈ ins ∧ ((x,y),r2) ∈ ins ⇒ r1 = r2) ∧
+    (∀x y r1 r2. ((x,y),r1) ∈ outs ∪ as ∧ ((x,y),r2) ∈ outs ∪ as ⇒ r1 = r2) ∧
+    (∀x y r. ((x,y),N,r) ∈ ins ⇒ (x,y-1) ∈ area) ∧
+    (∀x y r. ((x,y),S,r) ∈ ins ⇒ (x,y+1) ∈ area) ∧
+    (∀x y r. ((x,y),E,r) ∈ ins ⇒ (x+1,y) ∈ area) ∧
+    (∀x y r. ((x,y),W,r) ∈ ins ⇒ (x-1,y) ∈ area) ∧
+    (∀x y r. ((x,y),N,r) ∈ outs ⇒ (x,y+1) ∈ area) ∧
+    (∀x y r. ((x,y),S,r) ∈ outs ⇒ (x,y-1) ∈ area) ∧
+    (∀x y r. ((x,y),E,r) ∈ outs ⇒ (x-1,y) ∈ area) ∧
+    (∀x y r. ((x,y),W,r) ∈ outs ⇒ (x+1,y) ∈ area)
+End
+
+Definition circ_area_def:
+  circ_area area ins outs n =
+    if n MOD 60 < 30 then
+      base_area area DIFF
+      (U { io_box (x,y) | ∃d r. ((x,y),d,r) ∈ ins ∧ d ∈ {N;S} } ∪
+       U { io_box (x,y) | ∃d r. ((x,y),d,r) ∈ outs ∧ d ∈ {E;W} }) ∪
+      (U { io_box (x,y) | ∃d r. ((x,y),d,r) ∈ ins ∧ d ∈ {E;W} } ∪
+       U { io_box (x,y) | ∃d r. ((x,y),d,r) ∈ outs ∧ d ∈ {N;S} })
+    else
+      base_area area DIFF
+      (U { io_box (x,y) | ∃d r. ((x,y),d,r) ∈ ins ∧ d ∈ {E;W} } ∪
+       U { io_box (x,y) | ∃d r. ((x,y),d,r) ∈ outs ∧ d ∈ {N;S} }) ∪
+      (U { io_box (x,y) | ∃d r. ((x,y),d,r) ∈ ins ∧ d ∈ {N;S} } ∪
+       U { io_box (x,y) | ∃d r. ((x,y),d,r) ∈ outs ∧ d ∈ {E;W} })
+End
+
+Definition circ_io_area_def:
+  circ_io_area outs n =
+    if n MOD 60 = 29 then
+      U { io_box (x,y) | ∃r. ((x,y),r) ∈ outs ∧ x % 2 = 0 }
+    else if n MOD 60 = 59 then
+      U { io_box (x,y) | ∃r. ((x,y),r) ∈ outs ∧ x % 2 ≠ 0 }
+    else
+      {}
+End
+
+Definition io_gate_def:
+  io_gate E =
+   [[F;F;F;F;F;F;F;F;F;F];
+    [F;F;F;F;F;T;F;F;T;F];
+    [F;F;F;F;F;F;F;F;F;T];
+    [F;F;F;F;F;T;F;F;F;T];
+    [F;F;F;F;F;F;T;T;T;T];
+    [F;F;F;F;F;F;F;F;F;F];
+    [F;F;F;F;F;F;F;F;F;F];
+    [F;F;F;F;F;F;F;F;F;F];
+    [F;F;F;F;F;F;F;F;F;F];
+    [F;F;F;F;F;F;F;F;F;F]] ∧
+  io_gate W =
+   [[F;F;F;F;F;F;F;F;F;F];
+    [F;F;F;F;F;F;F;F;F;F];
+    [F;F;F;F;F;F;F;F;F;F];
+    [F;F;F;F;F;F;F;F;F;F];
+    [F;F;F;F;F;F;F;F;F;F];
+    [T;T;T;T;F;F;F;F;F;F];
+    [T;F;F;F;T;F;F;F;F;F];
+    [T;F;F;F;F;F;F;F;F;F];
+    [F;T;F;F;T;F;F;F;F;F];
+    [F;F;F;F;F;F;F;F;F;F]] ∧
+  io_gate N =
+   [[F;F;T;T;T;F;F;F;F;F];
+    [F;T;F;F;T;F;F;F;F;F];
+    [F;F;F;F;T;F;F;F;F;F];
+    [F;F;F;F;T;F;F;F;F;F];
+    [F;T;F;T;F;F;F;F;F;F];
+    [F;F;F;F;F;F;F;F;F;F];
+    [F;F;F;F;F;F;F;F;F;F];
+    [F;F;F;F;F;F;F;F;F;F];
+    [F;F;F;F;F;F;F;F;F;F];
+    [F;F;F;F;F;F;F;F;F;F]] ∧
+  io_gate S =
+   [[F;F;F;F;F;F;F;F;F;F];
+    [F;F;F;F;F;F;F;F;F;F];
+    [F;F;F;F;F;F;F;F;F;F];
+    [F;F;F;F;F;F;F;F;F;F];
+    [F;F;F;F;F;F;F;F;F;F];
+    [F;F;F;F;F;F;T;F;T;F];
+    [F;F;F;F;F;T;F;F;F;F];
+    [F;F;F;F;F;T;F;F;F;F];
+    [F;F;F;F;F;T;F;F;T;F];
+    [F;F;F;F;F;T;T;T;F;F]]
+End
+
+Definition from_row_def:
+  from_row (x,y) [] = {} ∧
+  from_row (x,y) (F::xs) = from_row (x+1:int,y:int) xs ∧
+  from_row (x,y) (T::xs) = {(x,y)} ∪ from_row (x+1,y) xs
+End
+
+Definition from_rows_def:
+  from_rows (x,y) [] = {} ∧
+  from_rows (x,y) (row :: rows) = from_row (x,y) row ∪ from_rows (x,y+1) rows
+End
+
+Definition lwss_as_set_def:
+  lwss_as_set (x,y) d = from_rows (x,y) (io_gate d)
+End
+
+Definition lwss_at_def:
+  lwss_at n ((x,y),d,r) =
+    if d ∈ {E; W} ∧ n MOD 60 = 59 ∧ r (n DIV 60) then
+      lwss_as_set (75 * x - 5, 75 * y - 5) d
+    else if d ∈ {N; S} ∧ n MOD 60 = 29 ∧ r (n DIV 60) then
+      lwss_as_set (75 * x - 5, 75 * y - 5) d
+    else
+      {}
+End
+
+Definition circ_io_lwss_def:
+  circ_io_lwss ins n = U (IMAGE (lwss_at n) ins )
+End
+
+Definition circ_mod_def:
+  circ_mod area ins outs as n =
+    <| area           := circ_area area ins outs n ;
+       deletions      := circ_io_area outs n ;
+       insertions     := circ_io_lwss ins n ;
+       assert_area    := circ_io_area (outs ∪ as) n ;
+       assert_content := circ_io_lwss (outs ∪ as) n |>
+End
+
+Theorem mods_wf_circ_mod:
+  circ_mod_wf area ins outs as ⇒
+  mods_wf (circ_mod area ins outs as)
+Proof
+  cheat
+QED
+
+Definition circuit_run_def:
+  circuit_run area ins outs as init ⇔
+    run (circ_mod area ins outs as) init ∧
+    circ_mod_wf area ins outs as
+End
+
+Definition circuit_def:
+  circuit area ins outs as init ⇔
+    circuit_run (set area) (set ins) (set outs) (set as) init ∧
+    ALL_DISTINCT area ∧
+    ALL_DISTINCT (MAP FST ins) ∧
+    ALL_DISTINCT (MAP FST outs) ∧
+    ALL_DISTINCT (MAP FST as)
+End
+
+Theorem run_to_le:
+  ∀k k0 c s t. run_to k c s t ∧ k0 ≤ k ⇒ ∃u. run_to k0 c s u
+Proof
+  cheat
+QED
+
+Theorem run_to_imp_run:
+  ∀k c s.
+    (∀n. ∃t. run_to (k * n) c s t) ∧ k ≠ 0 ⇒
+    run c s
+Proof
+  rw [run_def] \\ rename [‘run_to k1’]
+  \\ last_x_assum $ qspec_then ‘k1’ strip_assume_tac
+  \\ irule run_to_le
+  \\ pop_assum $ irule_at Any \\ gvs []
+QED
+
+Definition eval_io_def:
+  eval_io env ins =
+    MAP (λ((x,y),d,e). ((x,y),d, λn. eval (age n env) e)) ins
+End
+
+Theorem imp_circuit:
+  (∀env.
+    run_to 60
+      (circ_mod (set area)
+                (set (eval_io env ins))
+                (set (eval_io env outs))
+                {})
+      (from_rows (x,y) (MAP (MAP (eval env)) rows))
+      (from_rows (x,y) (MAP (MAP (eval (age 1 env))) rows)))
+  ⇒
+  circuit
+    area
+    (eval_io env ins)
+    (eval_io env ins)
+    []
+    (from_rows (x,y) (MAP (MAP (eval env)) rows))
+Proof
+  cheat
 QED
 
 
